stack machine compiler proofs

lectures/arith-to-stack-compiler.v
@@ -1,10 +1,19 @@
-From Coq Require Import Ascii String.
-From mathcomp Require Import ssreflect ssrfun ssrbool eqtype ssrnat seq.
 From Equations Require Import Equations.
+From QuickChick Require Import QuickChick.
+From mathcomp Require Import ssreflect ssrfun ssrbool eqtype ssrnat seq.
+From mathcomp Require Import zify.
+Import GenLow GenHigh.
+Set Warnings "-extraction-opaque-accessed,-extraction".
 
+Global Set Bullet Behavior "None".
 Set Implicit Arguments.
 Unset Strict Implicit.
 Unset Printing Implicit Defensive.
+
+(*| By default, the ``Equations`` plugin makes definitions opaque to avoid
+spurious unfoldings, but this behavior can be reverted using the following
+option. |*)
+Set Equations Transparent.
 
 (*|
 How to type Unicode notations in this file
@@ -40,6 +49,11 @@ functionality. |*)
      - `\ominus`
    * - `⊗`
      - `\otimes`
+   * - `⟿`
+     - `\longrightsquigarrow`
+   * - `⊞`
+     - `\boxplus`
+
 
 |*)
 
@@ -177,7 +191,7 @@ Equations run p s : stack :=
   run (⊗ :: p) (a1 :: a2 :: s) := run p ((a2 * a1) :: s);
   run _ s := s.
 
-
+Arguments run : simpl nomatch.
 
 (*| Unit and notation tests: |*)
 Check erefl : run [:: ⧐ 21; ⧐ 21; ⊕] [::] = [:: 42].
@@ -200,3 +214,173 @@ Equations compile e : prog :=
 
 Check erefl: run (compile ‴40 + 3 - 1‴) [::] = [:: 42].
 End Compiler.
+
+
+(*|
+Compiler correctness
+-------------------- |*)
+
+Import StackMachine.
+Import Compiler.
+
+Lemma compile_correct_generalized e s :
+  run (compile e) s = ⟦e⟧ :: s.
+Proof.
+elim: e s => //= e1 IH1 e2 IH2 s.
+(* At this point we might be looking for a way to utilize the induction
+hypotheses we just got. A lemma like ``run (p1 ++ p2) s = run p2 (run p1 s)``
+might seem intuitive, but before trying to prove it, let's see if we can get a
+counter-example using property-based randomized testing. *)
+Abort.
+
+
+Derive (Arbitrary, Show) for instr.
+
+Definition cat_run'_prop (p1 p2 : prog) (s : stack) :=
+  run (p1 ++ p2) s == run p2 (run p1 s).
+
+QuickChick cat_run'_prop.
+(*
+[Sub]
+[Push 0]
+[]
+*** Failed after 9 tests and 2 shrinks. (0 discards)
+*)
+
+(*| We got a counter-example right away! |*)
+
+(* We have several design choices here: either the stack-machine interpreter
+should signal a failure or we could add a typechecker for our stack language.
+Let's go with the latter approach. *)
+
+
+(* The type of a stack instruction / program *)
+Record stype : Type :=
+  mk_type {
+      (* min number of stack elements that needs be to present on the stack so
+      there is always a sufficient number of elements to proceed with
+      computation *)
+      inp : nat;
+      (* the number of elements the stack program produces overall *)
+      out : nat;
+    }.
+(* TODO: better names (notations?) for `inp` and `out` *)
+
+Implicit Type t : stype.
+
+Notation "i ⟿ o" := (mk_type i o) (at level 65, no associativity) : stack_scope.
+
+(*| The types of the stack instructions |*)
+Definition instr_type (i : instr) : stype :=
+  match i with
+  | ⧐ n => 0⟿1
+  | ⊕ | ⊖ | ⊗ => 2⟿1
+  end.
+
+(* combine (add) types of two consequtive instructions / programs *)
+(* Intuitively, `addst` is supposed to be a monoidial operation, see below *)
+Definition addst t1 t2 : stype :=
+  let: i1 ⟿ o1 := t1 in
+  let: i2 ⟿ o2 := t2 in
+  i1 + (i2 - o1) ⟿ o2 + (o1 - i2).
+
+Arguments addst : simpl nomatch.
+
+(* Nullary notation *)
+Notation "(⊞)" := (addst) : fun_scope.
+(* Binary infix notation *)
+Notation "s ⊞ t" := (addst s t) (at level 50, left associativity) : stack_scope.
+
+Lemma addtA : associative addst.
+Proof. case=> i1 o1 [i2 o2] [i3 o3] /=; congr mk_type; lia. Qed.
+
+Lemma add0t : left_id (0⟿0) addst.
+Proof. by case=> i o; rewrite /addst subn0 add0n sub0n addn0. Qed.
+
+Lemma addt0 : right_id (0⟿0) addst.
+Proof. by case=> i o; rewrite /addst subn0 add0n sub0n addn0. Qed.
+
+Lemma inpE t i o : inp ((i⟿o) ⊞ t) = i + (inp t - o).
+Proof. by case: t=> it ot /=. Qed.
+
+Definition infer (p : prog) : stype :=
+  foldr (fun i t => instr_type i ⊞ t) (0 ⟿ 0) p.
+
+Check erefl : infer [:: ⊖; ⊗] = 3⟿1.
+
+Lemma infer_cat : {morph infer : x y / x ++ y >-> x ⊞ y}.
+Proof.
+elim=> [[|i2 p2]| i1 p1 IHp1 p2] //=; first by rewrite add0t.
+by rewrite IHp1 addtA.
+Qed.
+
+(*| ``compile`` produces type-correct programs which do not consume any stack
+and put exactly one output value on the stack |*)
+Lemma infer_compile e :
+  infer (compile e) = 0⟿1.
+Proof.
+by elim: e => //= e1 IHe1 e2 IHe2; rewrite !infer_cat IHe1 IHe2.
+Qed.
+
+(*|
+Back to property based testing
+============================== |*)
+
+(* Using boolean implication, we can filter out incorrect stack programs when
+doing property based testing, let's also see some statistics showing how
+(in)efficient this is. *)
+Definition cat_run''_prop (p1 p2 : prog) (s : stack) :=
+  (inp (infer p1) <= size s) ==>
+  (run (p1 ++ p2) s == run p2 (run p1 s)).
+
+Extract Constant defNumTests => "10000".
+QuickChick (fun p1 p2 s =>
+  implication
+    (inp (infer p1) <= size s)
+    (run (p1 ++ p2) s == run p2 (run p1 s))).
+(* +++ Passed 10000 tests (1583 discards) *)
+
+(*| This is how one changes the number of QuickChick tests. |*)
+Extract Constant defNumTests => "11600".
+QuickChick (fun p1 p2 s =>
+  collect
+    (inp (infer p1) <= size s)
+    ((inp (infer p1) <= size s) ==> (run (p1 ++ p2) s == run p2 (run p1 s)))).
+(*
+7544 : true
+4056 : false
++++ Passed 11600 tests (0 discards)
+*)
+
+(* TODO: check the semantics of ``implication`` -- the results of
+``implication`` and ``collect`` are not in correspondence. Reported here:
+https://github.com/QuickChick/QuickChick/issues/228. *)
+
+(* TODO: show how to build a random generator producing type-correct stack programs *)
+
+
+
+(*|
+Back to proving
+=============== |*)
+Lemma run_cat p1 p2 s :
+  inp (infer p1) <= size s ->
+  run (p1 ++ p2) s = run p2 (run p1 s).
+Proof.
+elim: p1 s => // i1 p1 IHp1 s; case: i1=> [n | | |] /=.
+- rewrite inpE add0n=> Typ; rewrite IHp1 //=; lia.
+- rewrite inpE; case: s=> // e1 [//|e2 s /= T]; rewrite IHp1 //=; lia.
+- rewrite inpE; case: s=> // e1 [//|e2 s /= T]; rewrite IHp1 //=; lia.
+rewrite inpE; case: s=> // e1 [//|e2 s /= T]; rewrite IHp1 //=; lia.
+Qed.
+
+Lemma compile_correct_generalized e s :
+  run (compile e) s = ⟦e⟧ :: s.
+Proof.
+by elim: e s => //= e1 IH1 e2 IH2 s; rewrite !run_cat ?infer_compile // IH1 IH2.
+Qed.
+
+(*| The final correctness theorem |*)
+Lemma compile_correct e :
+  run (compile e) [::] = [:: ⟦e⟧].
+Proof. exact: compile_correct_generalized. Qed.
